expr.v, expr_lemmas.v - Some work on subset proofs semax_straight - definition for eventual "weak valid pointer" in pointer compare
floyd - added lemmas (no automation yet) for logical and and logical or. Uses a function
to represent the syntax.

floyd/forward.v
@@ -1,3 +1,4 @@
+Load loadpath.
 Require Import floyd.base.
 Require Import floyd.client_lemmas.
 Require Import floyd.field_mapsto.
@@ -21,6 +22,33 @@ The lemma goes here, because it imports from both forward_lemmas and call_lemmas
 
  See also BEGIN HORRIBLE1 , later in this file
 *)
+ 
+Definition logical_and_result v1 t1 v2 t2 :=
+match (strict_bool_val t1 v1) with
+| Some b1 => if b1 then match (strict_bool_val t2 v2) with
+                            | Some b2 => if b2 then  Vint Int.one 
+                                         else Vint Int.zero
+                            | None => Vundef end
+                   else Vint Int.zero
+| None => Vundef
+end.
+
+Definition logical_or_result v1 t1 v2 t2 :=
+match (strict_bool_val t1 v1) with
+| Some b1 => if b1 then Vint Int.one
+                   else match (strict_bool_val t2 v2) with
+                            | Some b2 => if b2 then  Vint Int.one 
+                                         else Vint Int.zero
+                            | None => Vundef end
+| None => Vundef
+end.
+
+Definition logical_or tid e1 e2 :=
+(Sifthenelse e1
+             (Sset tid (Econst_int (Int.repr 1) tint))
+             (Ssequence
+                (Sset tid (Ecast e2 tbool))
+                (Sset tid (Ecast (Etempvar tid tbool) tint)))).
 
 
 Definition logical_and tid e1 e2 :=
@@ -30,7 +58,6 @@ Definition logical_and tid e1 e2 :=
               (Sset tid (Ecast (Etempvar tid tbool) tint)))
             (Sset tid (Econst_int (Int.repr 0) tint))).
 
-(*
 Lemma semax_pre_flipped : 
  forall (P' : environ -> mpred) (Espec : OracleKind)
          (Delta : tycontext) (P1 : list Prop) (P2 : list (environ -> Prop))
@@ -43,6 +70,177 @@ Proof. intros.
 eapply semax_pre. apply H0. auto.
 Qed.
 
+Lemma tc_environ_init: forall Delta id rho,
+                         tc_environ (initialized id Delta) rho ->
+                         tc_environ Delta rho.
+Proof.  
+intros.
+unfold tc_environ in *. destruct Delta. destruct p. destruct p.
+unfold initialized in *. simpl in *. unfold temp_types in *.
+unfold var_types in *. unfold ret_type in *. simpl in *.
+remember (t1 ! id). destruct o; auto.
+destruct p. unfold typecheck_environ in *. intuition.
+clear - H0 Heqo. unfold typecheck_temp_environ in *.
+intros. destruct (eq_dec id id0). subst.
+specialize (H0 id0 true t3). spec H0.
+unfold temp_types in *. simpl in *. rewrite PTree.gss. auto.
+destruct H0. exists x. intuition. unfold temp_types in *.
+simpl in H. rewrite H in *. inv Heqo. auto.
+apply H0. 
+unfold temp_types in *. simpl in *.
+rewrite PTree.gso. auto. auto.
+Qed.
+
+Lemma bool_cast : forall e rho,
+   typecheck_val (eval_expr e rho) (typeof e) = true ->
+  eval_cast tbool tint (eval_cast (typeof e) tbool (eval_expr e rho)) =
+   match strict_bool_val (eval_expr e rho) (typeof e) with
+   | Some true => Vint Int.one
+   | Some false => Vint Int.zero
+   | None => Vundef
+   end.
+Proof.
+intros.
+unfold eval_cast. simpl.
+remember (eval_expr e rho). destruct v. inv H. simpl.
+ unfold eval_cast_neutral.
+remember (typeof e); destruct t; inv H; simpl;
+remember (Int.eq i Int.zero); if_tac; auto; try congruence.
+remember (typeof e); destruct t; inv H. simpl.
+if_tac; auto.
+destruct (typeof e); inv H; auto.
+Qed.
+
+Lemma semax_logical_or:
+ forall Espec Delta P Q R tid e1 e2 b
+   (CLOSQ : Forall (closed_wrt_vars (eq tid)) Q)
+   (CLOSR : Forall (closed_wrt_vars (eq tid)) R)
+   (CLOSE1 : closed_wrt_vars (eq tid) (eval_expr e1))
+   (CLOSE2 : closed_wrt_vars (eq tid) (eval_expr e2)),
+ bool_type (typeof e1) = true ->
+ bool_type (typeof e2) = true ->
+ (temp_types Delta) ! tid = Some (tint, b) ->
+  @semax Espec Delta (PROPx P (LOCALx ((tc_expr Delta e1)::(tc_expr Delta e2)::tc_temp_id tid tbool Delta (Ecast e2 tbool) ::
+   Q) (SEPx (R))))
+    (logical_or tid e1 e2)
+  (normal_ret_assert (PROPx P (LOCALx 
+((`eq (eval_id tid) 
+   (`logical_or_result 
+          `(typeof e1) (eval_expr e1) `(typeof e2) (eval_expr e2)))::Q) (SEPx (R))))). 
+Proof.
+intros.
+apply semax_ifthenelse_PQR. 
+  - auto. 
+  -  eapply semax_pre. apply derives_refl.
+     eapply semax_post_flipped.
+     apply forward_setx. 
+     intro rho. normalize. apply prop_right. simpl.
+     unfold tc_temp_id. unfold typecheck_temp_id. rewrite H1.
+     simpl. auto.
+     intros ek vl rho. normalize. apply normal_ret_assert_derives'.
+     apply exp_left. intro old. normalize. autorewrite with subst.
+     intro rho'. normalize.
+     repeat apply andp_right; normalize. apply prop_right.
+     unfold logical_or_result. unfold typed_true in *.
+     unfold subst in *. 
+
+     assert ((eval_expr e1 (env_set rho' tid old)) =
+                  eval_expr e1 rho').
+              replace rho' with (mkEnviron (ge_of rho') (ve_of rho')
+                                         (te_of rho')).
+              unfold env_set. simpl.
+              erewrite <- CLOSE1. destruct rho'. simpl. auto.
+              intros. rewrite Map.gsspec. if_tac; auto. destruct rho'; 
+                                                        auto.
+     
+     super_unfold_lift. rewrite H10 in *. clear H10.
+     rewrite H6. simpl. rewrite H4. simpl. super_unfold_lift.
+     auto.
+  - eapply semax_seq'. 
+      + eapply forward_setx.
+        intro rho. normalize. 
+        apply andp_right; apply prop_right.
+        unfold tc_expr. simpl. rewrite tc_andp_sound.
+        simpl. super_unfold_lift. split. auto. 
+        unfold isCastResultType. simpl. destruct (typeof e2); 
+                                        inv H0; simpl; auto.
+        simpl.  auto.
+      + simpl update_tycon. apply extract_exists_pre. intro oldval.
+        autorewrite with subst.  
+        apply (semax_pre ((PROPx P
+        (LOCALx
+           (tc_environ (initialized tid Delta) ::
+             `eq (eval_id tid) (eval_expr (Ecast e2 tbool))
+            :: `(typed_false (typeof e1)) (eval_expr e1)
+               :: tc_expr Delta e2
+                  :: Q)
+           (SEPx R))))). intro rho. normalize.
+        eapply semax_post_flipped.
+        eapply forward_setx. intro rho. normalize.
+        apply andp_right; apply prop_right. 
+        unfold tc_expr. simpl. rewrite tc_andp_sound. 
+        super_unfold_lift. split. 
+        erewrite temp_types_init_same by eauto. simpl. auto.
+        simpl. auto.
+        simpl. unfold tc_temp_id. unfold typecheck_temp_id.
+        erewrite temp_types_init_same by eauto. rewrite tc_andp_sound.
+        simpl. super_unfold_lift; auto.
+        intros. intro rho.
+        normalize. apply normal_ret_assert_derives'.
+        apply exp_left. intro old. autorewrite with subst.
+        intro rho'. normalize. repeat apply andp_right; 
+                               [ | normalize | normalize].
+
+        { apply prop_right.
+          rewrite H4. simpl. super_unfold_lift.
+          simpl. unfold subst in *.
+          unfold eval_id. simpl. rewrite Map.gss. simpl.
+          apply expr_lemmas.typecheck_expr_sound in H8.
+          Focus 2. eapply tc_environ_init. apply H5.
+
+
+          assert ((eval_expr (Ecast e2 tbool) (env_set rho' tid old)) =
+                  eval_expr (Ecast e2 tbool) rho').
+              simpl. super_unfold_lift. unfold eval_cast. simpl.
+              remember (typeof e2). 
+              replace rho' with (mkEnviron (ge_of rho') (ve_of rho')
+                                         (te_of rho')).
+              unfold env_set. simpl.
+              erewrite <- CLOSE2. destruct rho'. simpl. auto.
+              intros. rewrite Map.gsspec. if_tac; auto. destruct rho'; 
+                                                        auto.
+          rewrite H10 in *. simpl in H10. super_unfold_lift.
+          clear H9 H10. rewrite H6.
+          assert ((eval_expr e2 (env_set rho' tid old)) =
+                  eval_expr e2 rho').
+              replace rho' with (mkEnviron (ge_of rho') (ve_of rho')
+                                         (te_of rho')).
+              unfold env_set. simpl.
+              erewrite <- CLOSE2. destruct rho'. simpl. auto.
+              intros. rewrite Map.gsspec. if_tac; auto. destruct rho'; 
+                                                        auto.
+          rewrite H9 in *. clear H9.
+          assert ((eval_expr e1 (env_set rho' tid old)) =
+                  eval_expr e1 rho').
+              replace rho' with (mkEnviron (ge_of rho') (ve_of rho')
+                                         (te_of rho')).
+              unfold env_set. simpl.
+              erewrite <- CLOSE1. destruct rho'. simpl. auto.
+              intros. rewrite Map.gsspec. if_tac; auto. destruct rho'; 
+                                                        auto.
+          rewrite H9 in *.
+          clear H4 H6 H9 H3. 
+          simpl. super_unfold_lift.
+          unfold logical_or_result. 
+          unfold typed_false in *. rewrite H7.
+          simpl. 
+          apply bool_cast. auto.
+          }
+Qed.
+
+
+
+
 Lemma semax_logical_and:
  forall Espec Delta P Q R tid e1 e2 b
    (CLOSQ : Forall (closed_wrt_vars (eq tid)) Q)
@@ -52,72 +250,139 @@ Lemma semax_logical_and:
  bool_type (typeof e1) = true ->
  bool_type (typeof e2) = true ->
  (temp_types Delta) ! tid = Some (tint, b) ->
-  @semax Espec Delta (PROPx P (LOCALx ((tc_expr Delta e1)::(tc_expr Delta e2)::
+  @semax Espec Delta (PROPx P (LOCALx ((tc_expr Delta e1)::(tc_expr Delta e2)::tc_temp_id tid tbool Delta (Ecast e2 tbool) ::
    Q) (SEPx (R))))
     (logical_and tid e1 e2)
-  (normal_ret_assert (PROPx P (LOCALx Q (SEPx (R)))))
+  (normal_ret_assert (PROPx P (LOCALx 
+((`eq (eval_id tid) 
+   (`logical_and_result 
+          `(typeof e1) (eval_expr e1) `(typeof e2) (eval_expr e2)))::Q) (SEPx (R)))))
   . 
 Proof.
 intros.
-eapply semax_post_flipped.
 apply semax_ifthenelse_PQR. 
-auto. 
-eapply semax_post_flipped.
-eapply semax_seq'.
-eapply semax_pre_flipped.
-apply forward_setx_closed_now.
-Focus 6. apply derives_refl.
-Focus 6. instantiate (1:=R). 
-intro rho. 
-instantiate (1:= 
-        (`(typed_true (typeof e1)) (eval_expr e1)
-            :: tc_expr Delta e2 :: Q)).
-normalize.
-auto 50 with closed. 
-auto 50 with closed.
-auto with closed.
-intro rho. normalize. 
-apply prop_right.
-clear H4. 
-unfold tc_expr in *. simpl. 
-rewrite tc_andp_sound. simpl. 
-super_unfold_lift. split.
-auto. destruct (typeof e2); try inv H0; simpl; auto. 
+  - auto. 
+  - eapply semax_seq'. 
+      + eapply forward_setx.
+        intro rho. normalize. 
+        apply andp_right; apply prop_right.
+        unfold tc_expr. simpl. rewrite tc_andp_sound.
+        simpl. super_unfold_lift. split. auto. 
+        unfold isCastResultType. simpl. destruct (typeof e2); 
+                                        inv H0; simpl; auto.
+        simpl.  auto.
+      + simpl update_tycon. apply extract_exists_pre. intro oldval.
+        autorewrite with subst.  
+        apply (semax_pre ((PROPx P
+        (LOCALx
+           (tc_environ (initialized tid Delta) ::
+             `eq (eval_id tid) (eval_expr (Ecast e2 tbool))
+            :: `(typed_true (typeof e1)) (eval_expr e1)
+               :: tc_expr Delta e2
+                  :: Q)
+           (SEPx R))))). intro rho. normalize.
+        eapply semax_post_flipped.
+        eapply forward_setx. intro rho. normalize.
+        apply andp_right; apply prop_right. 
+        unfold tc_expr. simpl. rewrite tc_andp_sound. 
+        super_unfold_lift. split. 
+        erewrite temp_types_init_same by eauto. simpl. auto.
+        simpl. auto.
+        simpl. unfold tc_temp_id. unfold typecheck_temp_id.
+        erewrite temp_types_init_same by eauto. rewrite tc_andp_sound.
+        simpl. super_unfold_lift; auto.
+        intros. intro rho.
+        normalize. apply normal_ret_assert_derives'.
+        apply exp_left. intro old. autorewrite with subst.
+        intro rho'. normalize. repeat apply andp_right; 
+                               [ | normalize | normalize].
 
-intro rho. normalize. apply prop_right.
-simpl. unfold tc_temp_id. 
-unfold typecheck_temp_id. 
-rewrite H1. simpl; auto. 
+        { apply prop_right.
+          rewrite H4. simpl. super_unfold_lift.
+          simpl. unfold subst in *.
+          unfold eval_id. simpl. rewrite Map.gss. simpl.
+          apply expr_lemmas.typecheck_expr_sound in H8.
+          Focus 2. eapply tc_environ_init. apply H5.
 
-apply temp_types_init_same in H1.
-apply forward_setx.
-intro rho. normalize. apply andp_right;
-apply prop_right. 
-simpl. 
-unfold tc_expr in *. simpl. 
-rewrite tc_andp_sound. simpl.
-clear H5.  
-super_unfold_lift. split; auto. 
- rewrite H1.
-compute; auto. 
 
-simpl. unfold tc_temp_id. unfold typecheck_temp_id.
-rewrite H1. simpl. auto.
+          assert ((eval_expr (Ecast e2 tbool) (env_set rho' tid old)) =
+                  eval_expr (Ecast e2 tbool) rho').
+              simpl. super_unfold_lift. unfold eval_cast. simpl.
+              remember (typeof e2). 
+              replace rho' with (mkEnviron (ge_of rho') (ve_of rho')
+                                         (te_of rho')).
+              unfold env_set. simpl.
+              erewrite <- CLOSE2. destruct rho'. simpl. auto.
+              intros. rewrite Map.gsspec. if_tac; auto. destruct rho'; 
+                                                        auto.
+          rewrite H10 in *. simpl in H10. super_unfold_lift.
+          clear H9 H10. rewrite H6.
+          assert ((eval_expr e2 (env_set rho' tid old)) =
+                  eval_expr e2 rho').
+              replace rho' with (mkEnviron (ge_of rho') (ve_of rho')
+                                         (te_of rho')).
+              unfold env_set. simpl.
+              erewrite <- CLOSE2. destruct rho'. simpl. auto.
+              intros. rewrite Map.gsspec. if_tac; auto. destruct rho'; 
+                                                        auto.
+          rewrite H9 in *. clear H9.
+          assert ((eval_expr e1 (env_set rho' tid old)) =
+                  eval_expr e1 rho').
+              replace rho' with (mkEnviron (ge_of rho') (ve_of rho')
+                                         (te_of rho')).
+              unfold env_set. simpl.
+              erewrite <- CLOSE1. destruct rho'. simpl. auto.
+              intros. rewrite Map.gsspec. if_tac; auto. destruct rho'; 
+                                                        auto.
+          rewrite H9 in *.
+          clear H4 H6 H9 H3. 
+          simpl. super_unfold_lift.
+          unfold logical_and_result. 
+          unfold typed_true in *. rewrite H7.
+          simpl. 
 
-Focus 2. 
-eapply semax_post_flipped.
+        apply bool_cast. auto. }
+  -  eapply semax_pre. apply derives_refl.
+     eapply semax_post_flipped.
+     apply forward_setx. 
+     intro rho. normalize. apply prop_right. simpl.
+     unfold tc_temp_id. unfold typecheck_temp_id. rewrite H1.
+     simpl. auto.
+     intros ek vl rho. normalize. apply normal_ret_assert_derives'.
+     apply exp_left. intro old. normalize. autorewrite with subst.
+     intro rho'. normalize.
+     repeat apply andp_right; normalize. apply prop_right.
+     unfold logical_and_result. unfold typed_false in *.
+     unfold subst in *. 
 
-eapply semax_pre_flipped.
-apply forward_setx_closed_now.
-Focus 7. 
-instantiate (1:=R).
-instantiate (1:=`(typed_false (typeof e1)) (eval_expr e1)
-            :: tc_expr Delta e2 :: Q).
-intro rho. 
-normalize. 
-intros.  
-
-Focus *)
+     assert ((eval_expr e1 (env_set rho' tid old)) =
+                  eval_expr e1 rho').
+              replace rho' with (mkEnviron (ge_of rho') (ve_of rho')
+                                         (te_of rho')).
+              unfold env_set. simpl.
+              erewrite <- CLOSE1. destruct rho'. simpl. auto.
+              intros. rewrite Map.gsspec. if_tac; auto. destruct rho'; 
+                                                        auto.
+     
+     super_unfold_lift. rewrite H10 in *. clear H10.
+     rewrite H6. simpl. rewrite H4. simpl. super_unfold_lift.
+     assert (exists v, strict_bool_val (eval_expr e2 rho') (typeof e2) = Some v).
+     assert ((eval_expr e2 (env_set rho' tid old)) =
+                  eval_expr e2 rho').
+              replace rho' with (mkEnviron (ge_of rho') (ve_of rho')
+                                         (te_of rho')).
+              unfold env_set. simpl.
+              erewrite <- CLOSE2. destruct rho'. simpl. auto.
+              intros. rewrite Map.gsspec. if_tac; auto. destruct rho'; 
+                                                        auto.
+     apply expr_lemmas.typecheck_expr_sound in H7; auto.
+     rewrite H10 in *. remember (eval_expr e2 rho'). 
+     destruct v; eauto; 
+     destruct (typeof e2); simpl; eauto; try solve[inv H7; 
+     try rewrite H12; eauto]; simpl in *; congruence.
+     auto.
+Qed.
+     
 
 
 Lemma semax_call_id1_x:
@@ -726,13 +991,35 @@ Ltac is_canonical P :=
  | _ => fail 2 "precondition is not canonical (PROP _ LOCAL _ SEP _)"
  end.
 
-Lemma is_ptr_type: forall t, (tptr t = tptr t).
-Proof. reflexivity. Qed.
+Ltac bool_compute b :=
+let H:= fresh in 
+  assert (b=true) as H by auto; clear H. 
 
-Ltac is_ptr_type t := let H:=fresh in assert (H:t=t) by apply is_ptr_type; clear H.
+Ltac tac_if b T F := 
+first [bool_compute b;T | F].
 
-Ltac ptr_compare_tac := fail 2 "ptr_compare_tac not implemented".
-  
+Definition ptr_compare e :=
+match e with
+| (Ebinop cmp e1 e2 ty) =>
+   andb (andb (is_comparison cmp) (is_pointer_type (typeof e1))) (is_pointer_type (typeof e2))
+| _ => false
+end.
+
+
+Ltac forward_ptr_cmp := 
+first [eapply forward_ptr_compare_closed_now;
+       [    solve [auto 50 with closed] 
+          | solve [auto 50 with closed] 
+          | solve [auto 50 with closed] 
+          | solve [auto 50 with closed]
+          | 
+          | reflexivity ]
+       | eapply forward_ptr_compare'; try reflexivity].
+ 
+Ltac forward_setx_with_pcmp e :=
+tac_if (ptr_compare e) ltac:forward_ptr_cmp ltac:forward_setx.
+
+
 Ltac forward1 :=   
    match goal with |- @semax _ _ (PROPx _ (LOCALx _ (SEPx _))) _ _ => idtac 
        | |- _ => fail 2 "precondition is not canonical (PROP _ LOCAL _ SEP _)"
@@ -746,11 +1033,8 @@ Ltac forward1 :=
          semax_field_tac || fail 2 "semax_field_tac failed"
   | |- @semax _ _ _ (Sset _ (Ederef _ _)) _ => 
          load_array_tac || fail 2 "load_array_tac failed"
-  | |- @semax _ _ _ (Sset _ (Ebinop _ ?e1 _ _)) _ => 
-                is_ptr_type (typeof e1); 
-                first [ptr_compare_tac | fail 2 "ptr_compare_tac failed"]
   | |- @semax _ _ _ (Sset ?id ?e) _ => 
-          forward_setx || fail 2 "forward_setx failed"
+          forward_setx_with_pcmp e || fail 2 "forward_setx failed"
   | |- @semax _ ?Delta (PROPx ?P (LOCALx ?Q ?R)) 
                                  (Sifthenelse ?e _ _) _ =>
             (apply semax_pre
@@ -768,6 +1052,7 @@ Ltac forward1 :=
                    semax_call_id_tac_aux Espec Delta P Q R id f bl
 *)
   end.
+
 
 Ltac forward0 :=  (* USE FOR DEBUGGING *)
   match goal with 
